---
title: 4 - relaxing the proof style.md
description: 
published: true
date: 2023-08-19T23:27:59.086Z
tags: 
editor: markdown
dateCreated: 2023-07-04T04:11:36.454Z
---

![](/images/20220922093241.png)
- *Monotonicity* if $(x \Rightarrow y) \Rightarrow (f(x) \Rightarrow f(y))$

> ***Prove (4.2)***
> ![](/images/20220922094540.png)
> ![](/images/20220922094556.png)
> Starting with the consequence, we were forced to use $\Leftarrow$. Starting with the antecedent, we can use $\Rightarrow$.

> ***Deduction Theorem***
> Suppose adding $P_1, \dots, P_n$ as axioms to propositional logic, with the variables of the $P_i$ considered to be constants, allows $Q$ to be proved. Then $P_1 \land \dots \land P_n \Rightarrow Q$ is a theorem.


